examples of switch fail; corrected join postondition of switch + proof for modified version of code

doc/tutorial/C/switch.c
@@ -1,12 +1,24 @@
-int switch_test(int i) {
+int switch_test (int i) {
   
     switch(i) {
     case 0:
-       return 0 ; break;
+       return 0; 
     case 1:
-      return 1 ; break;
-    default : return 2;
+      return 0;
+    default : break;
     }
+    return 0;
+}
+
+int switch_test_fail (int i) {
+  
+    switch(i) {
+    case 0:
+       return 0;
+    case 1:
+      return 0;
+    }
+    return 0;
 }
 
 int twice (int n) {
@@ -14,14 +26,20 @@ int twice (int n) {
   case 0: return 0;
   case 1: n=2; return n;
   case -1: n= -2; return n;
-  // case 3: n=n+0;
-  // default: n=n+n; break;
+  case 3: n=n+0; /* Fall Through */
+  default: n=n+n; break;
   }
-  return n + n;
+  return n;
 }
 
-int f(unsigned int x) { switch (x) {
-   case 1: return 2; break;
-   case 2: case 3: case 0xffffffff: return 1; break;
-   default: return 1; }
+int twice_fail (int n) {
+  switch (n) {
+  case 0: return 0;
+  case 1: n=2; return n;
+  case -1: n= -2; return n; 
+  case 3: n=n+0; /* Fall Through */
+  // default: n=n+n; break;
+  }
+  n = n + n;
+  return n;
 }
