doc/tutorial/vst_switch.v
@@ -15,34 +15,45 @@ Definition switch_spec : ident * funspec :=
       SEP()
     POST [ tint ]
       PROP()
-      LOCAL(temp ret_temp (if Int.eq i Int.zero
-                           then Vint Int.zero
-                           else if Int.eq i Int.one
-                                then Vint Int.one
-                                else Vint (Int.repr 2)))
-                 SEP().
+      LOCAL(temp ret_temp (Vint (Int.repr 0)))
+      SEP().
 
 Definition Gprog := ltac:(with_library prog [switch_spec]).
 
-     
-Lemma body_max: semax_body Vprog Gprog f_switch_test switch_spec.
-Proof.
-  start_function.
-  forward_if ((@FF (environ->mpred) _));
-    forward; try entailer!.  
-  - replace (Int.eq i Int.zero) with true.
-    auto.
-    rewrite Int.signed_eq.
-    destruct zeq; intuition.
-  - repeat rewrite Int.signed_eq.
-    destruct zeq; intuition; simpl.
-    replace (Int.signed Int.zero) with 0 in * by auto with ints.
-    intuition.
-    destruct zeq; intuition.
-  - admit.
-Admitted.
+Lemma body_switch_test: semax_body Vprog Gprog f_switch_test switch_spec.
+ Proof.
+   start_function.
+   forward_if True.
+   repeat forward.
+   forward.
+   forward.
+   entailer!.
+   forward.
+Qed.
 
-Require Import Clight.switch.
+Definition switch_fail_spec : ident * funspec :=
+  DECLARE _switch_test_fail
+    WITH i : int
+    PRE [_i OF tint]
+      PROP()
+      LOCAL(temp _i (Vint (Int.repr (Int.signed i))))
+      SEP()
+    POST [ tint ]
+      PROP()
+      LOCAL(temp ret_temp (Vint (Int.repr 0)))
+      SEP().
+
+Definition Gprog_switch := ltac:(with_library prog [switch_fail_spec]).
+
+Lemma body_switch_fail_test: semax_body Vprog Gprog_switch f_switch_test_fail switch_fail_spec.
+ Proof.
+   start_function.
+   forward_if True.
+   repeat forward.
+   forward.
+   forward.
+   entailer!.
+Abort.
 
 Definition twice_spec :=
   DECLARE _twice
@@ -56,43 +67,41 @@ Definition twice_spec :=
       LOCAL (temp ret_temp (Vint (Int.repr (n+n))))
       SEP ().
 
-
-Definition f_spec :=
-  DECLARE _f
-    WITH x : Z
-    PRE [ _x OF tuint ]
-      PROP  (0 <= x <= Int.max_unsigned)
-      LOCAL (temp _x (Vint (Int.repr x)))
-      SEP ()
-    POST [ tint ]
-      PROP ()
-      LOCAL (temp ret_temp (if (x =? 1) 
-                            then Vint (Int.repr 2) 
-                            else Vint (Int.repr 1)))
-      SEP ().
-
-
 Definition Gprog' : funspecs :=   ltac:(with_library prog [twice_spec]).
 
 Lemma body_twice: semax_body Vprog Gprog' f_twice twice_spec.
+Proof.
+start_function.
+forward_if (PROP() LOCAL(temp _n (Vint (Int.repr (n + n)))) SEP()).
+repeat forward; entailer!.
+repeat forward; entailer!.
+repeat forward; entailer!.
+repeat forward; entailer!.
+repeat forward; entailer!.
+repeat forward; entailer!.
+Qed.
+
+Definition twice_fail_spec :=
+  DECLARE _twice_fail
+    WITH n : Z
+    PRE [ _n OF tint ]
+      PROP  (Int.min_signed <= n+n <= Int.max_signed)
+      LOCAL (temp _n (Vint (Int.repr n)))
+      SEP ()
+    POST [ tint ]
+      PROP ()
+      LOCAL (temp ret_temp (Vint (Int.repr (n+n))))
+      SEP ().
+
+Definition Gprog'' : funspecs :=   ltac:(with_library prog [twice_fail_spec]).
+
+Lemma body_twice_fail: semax_body Vprog Gprog'' f_twice_fail twice_fail_spec.
 Proof.
 start_function.
 forward_if (PROP() LOCAL(temp _n (Vint (Int.repr (n)))) SEP()).
 repeat forward; entailer!.
 repeat forward; entailer!.
 repeat forward; entailer!.
-repeat forward; entailer!.
-repeat forward; entailer!.
-repeat forward; entailer!.
-Qed.
-
-Lemma body_f: semax_body Vprog Gprog f_f f_spec.
-Proof.
-start_function.
-forward_if (@FF (environ->mpred) _).
 forward.
-forward.
-forward.
-forward.
-forward.
-Qed.
+entailer.
+Abort.
